Some file reorganization. Eliminate the propositional logic's dependency on syntactic reduction.

LogicBase.v
@@ -14,15 +14,6 @@ Fixpoint propagation_denote {L: Language} (p: list single_propagation) (x: expr)
   | sp :: p0 => single_propagation_denote sp (propagation_denote p0 x)
   end.
 
-Class NormalLanguage (L: Language): Type := {
-  falsep: expr;
-  impp: expr -> expr -> expr;
-  imp1_propag: expr -> single_propagation;
-  imp2_propag: expr -> single_propagation;
-  imp1_propag_denote: forall x y, single_propagation_denote (imp1_propag x) y = impp y x;
-  imp2_propag_denote: forall x y, single_propagation_denote (imp2_propag x) y = impp x y
-}.
-
 Definition context {L: Language}: Type := Ensemble expr.
 
 Definition empty_context {L: Language}: context := Empty_set _.
@@ -32,27 +23,14 @@ Class ProofTheory (L: Language): Type := {
   derivable: context -> expr -> Prop
 }.
 
-Definition multi_imp {L: Language} {nL: NormalLanguage L} (xs: list expr) (y: expr): expr :=
-  fold_right impp y xs.
-
-Class NormalProofTheory (L: Language) {nL: NormalLanguage L} (Gamma: ProofTheory L): Type := {
-  derivable_provable: forall Phi y, derivable Phi y <->
-                        exists xs, Forall (fun x => Phi x) xs /\ provable (multi_imp xs y)
-}.
-
-Definition consistent {L: Language} {nL: NormalLanguage L} {Gamma: ProofTheory L}: context -> Prop :=
-  fun Phi => ~ derivable Phi falsep.
-
-Definition maximal_consistent {L: Language} {nL: NormalLanguage L} {Gamma: ProofTheory L}: context -> Prop :=
-  fun Phi => consistent Phi /\ forall Psi, consistent Psi -> Included _ Phi Psi -> Included _ Psi Phi.
-
-Definition derivable_closed {L: Language} {nL: NormalLanguage L} {Gamma: ProofTheory L}: context -> Prop :=
-  fun Phi => forall x, derivable Phi x -> Phi x.
-
 Class Semantics (L: Language): Type := {
   model: Type;
   satisfies: model -> expr -> Prop
 }.
+
+Definition consistent {L: Language} {Gamma: ProofTheory L}: context -> Prop :=
+  fun Phi =>
+    exists x: expr, ~ derivable Phi x.
 
 Definition consequence {L: Language} {SM: Semantics L}: context -> expr -> Prop :=
   fun Phi y =>
@@ -81,116 +59,4 @@ Notation "Phi  |==  x" := (consequence Phi x) (at level 60, no associativity) : 
 Notation "|--  x" := (provable x) (at level 61, no associativity) : logic_base.
 Notation "Phi  |--  x" := (derivable Phi x) (at level 60, no associativity) : logic_base.
 
-(* Properties *)
-
-Local Open Scope logic_base.
-
-Lemma provable_derivable {L: Language} {nL: NormalLanguage L} {Gamma: ProofTheory L} {nGamma: NormalProofTheory L Gamma}: forall x, provable x <-> derivable empty_context x.
-Proof.
-  intros.
-  rewrite derivable_provable.
-  split; intros.
-  + exists nil; split; auto.
-  + destruct H as [xs [? ?]].
-    destruct xs; [auto |].
-    inversion H; subst.
-    inversion H3.
-Qed.  
-
-Lemma derivable_weaken {L: Language} {nL: NormalLanguage L} {Gamma: ProofTheory L} {nGamma: NormalProofTheory L Gamma}: forall Phi Psi x,
-  Included _ Phi Psi ->
-  Phi |-- x ->
-  Psi |-- x.
-Proof.
-  intros.
-  rewrite derivable_provable in H0 |- *.
-  destruct H0 as [xs [? ?]].
-  exists xs; split; auto.
-  revert H0; apply Forall_impl.
-  auto.
-Qed.
-
-Lemma derivable_weaken1 {L: Language} {nL: NormalLanguage L} {Gamma: ProofTheory L} {nGamma: NormalProofTheory L Gamma}: forall Phi x y,
-  Phi |-- y ->
-  Union _ Phi (Singleton _ x) |-- y.
-Proof.
-  intros.
-  eapply derivable_weaken; eauto.
-  intros ? ?; left; auto.
-Qed.
-
-Lemma impp_intros {L: Language} {nL: NormalLanguage L} {Gamma: ProofTheory L} {nGamma: NormalProofTheory L Gamma}: forall Phi x y,
-  Phi |-- impp x y ->
-  Union _ Phi (Singleton _ x) |-- y.
-Proof.
-  intros.
-  rewrite derivable_provable in H |- *.
-  destruct H as [xs [? ?]].
-  exists (xs ++ (x :: nil)).
-  split.
-  + rewrite Forall_app_iff; split.
-    - revert H; apply Forall_impl.
-      intros.
-      left; auto.
-    - constructor; auto.
-      right. constructor.
-  + replace (multi_imp (xs ++ x :: nil) y) with (multi_imp xs (impp x y)); auto.
-    clear.
-    induction xs; auto.
-    simpl; f_equal; auto.
-Qed.
-
-Lemma maximal_consistent_spec {L: Language} {nL: NormalLanguage L} {Gamma: ProofTheory L} {nGamma: NormalProofTheory L Gamma}:
-  forall Phi, maximal_consistent Phi <-> consistent Phi /\ forall x, consistent (Union _ Phi (Singleton _ x)) -> Phi x.
-Proof.
-  intros.
-  split; intros [? ?]; split; auto.
-  + intros.
-    specialize (H0 _ H1).
-    specialize (H0 (fun x H => Union_introl _ _ _ _ H)).
-    specialize (H0 x).
-    apply H0; right; constructor.
-  + intros.
-    hnf; intros.
-    apply H0.
-    unfold consistent in*.
-    intro; apply H1.
-    eapply derivable_weaken; [| exact H4].
-    intros ? [? | ?]; auto.
-    intros []; auto.
-Qed.
-
-Module AxiomaticProofTheory.
-
-Class AxiomaticProofTheory (L: Language): Type := {
-  provable: expr -> Prop
-}.
-
-Definition derivable {L: Language} {nL: NormalLanguage L} {Gamma: AxiomaticProofTheory L}: context -> expr -> Prop :=
-  fun Phi y =>
-    exists xs, Forall (fun x => Phi x) xs /\ provable (multi_imp xs y).
-
-Instance G {L: Language} {nL: NormalLanguage L} (Gamma: AxiomaticProofTheory L): ProofTheory L :=
-  Build_ProofTheory L provable derivable.
-
-Instance nG {L: Language} {nL: NormalLanguage L} (Gamma: AxiomaticProofTheory L): NormalProofTheory L (G Gamma) :=
-  Build_NormalProofTheory L nL (G Gamma) (fun _ _ => iff_refl _).
-
-End AxiomaticProofTheory.
-
-Module SequentCalculus.
-
-Class ProofTheory (L: Language): Type := {
-  derivable: context -> expr -> Prop
-}.
-
-Definition provable {L: Language} {Gamma: ProofTheory L}: expr -> Prop :=
-  fun x => derivable (Empty_set _) x.
-
-(*
-Instance SequentCalculus {L: Language} (Gamma: SequentCalculus.ProofTheory L): ProofTheory L :=
-  Build_ProofTheory L SequentCalculus.provable SequentCalculus.derivable (fun x => iff_refl _).
-*)
-
-End SequentCalculus.
 
