PropositionalLogic/ClassicalPropositionalLogic.v
@@ -1,19 +1,20 @@
 Require Import Coq.Logic.Classical_Prop.
 Require Import Logic.lib.Coqlib.
 Require Import Logic.LogicBase.
-Require Import Logic.SyntacticReduction.
+Require Import Logic.MinimunLogic.MinimunLogic.
+Require Import Logic.MinimunLogic.SyntacticReduction.
+Require Import Logic.MinimunLogic.ContextProperty.
 Require Import Logic.PropositionalLogic.Syntax.
-Require Import Logic.PropositionalLogic.MinimunPropositionalLogic.
 
 Local Open Scope logic_base.
 Local Open Scope PropositionalLogic.
 
-Class ClassicalPropositionalLogic (L: Language) {nL: NormalLanguage L} {pL: PropositionalLanguage L} (Gamma: ProofTheory L) {mpGamma: MinimunPropositionalLogic L Gamma} {rcGamma: ReductionConsistentProofTheory MendelsonReduction Gamma} := {
+Class ClassicalPropositionalLogic (L: Language) {nL: NormalLanguage L} {pL: PropositionalLanguage L} (Gamma: ProofTheory L) {mpGamma: MinimunPropositionalLogic L Gamma} := {
   axiom3: forall x y, |-- ((~~ y --> x) --> (~~ y --> ~~ x) --> y);
   true_provable: provable TT
 }.
 
-Lemma axiom3_derivable: forall {L: Language} {nL: NormalLanguage L} {pL: PropositionalLanguage L} {Gamma: ProofTheory L} {nGamma: NormalProofTheory L Gamma} {mpGamma: MinimunPropositionalLogic L Gamma} {rcGamma: ReductionConsistentProofTheory MendelsonReduction Gamma} {cpGamma: ClassicalPropositionalLogic L Gamma} (Phi: context) (x y: expr),
+Lemma axiom3_derivable: forall {L: Language} {nL: NormalLanguage L} {pL: PropositionalLanguage L} {Gamma: ProofTheory L} {nGamma: NormalProofTheory L Gamma} {mpGamma: MinimunPropositionalLogic L Gamma} {cpGamma: ClassicalPropositionalLogic L Gamma} (Phi: context) (x y: expr),
   Phi |-- (~~ x --> y) --> (~~ x --> ~~ y) --> x.
 Proof.
   intros.
@@ -23,7 +24,7 @@ Proof.
   intros ? [].
 Qed.
 
-Lemma contradiction_rule: forall {L: Language} {nL: NormalLanguage L} {pL: PropositionalLanguage L} {Gamma: ProofTheory L} {nGamma: NormalProofTheory L Gamma} {mpGamma: MinimunPropositionalLogic L Gamma} {rcGamma: ReductionConsistentProofTheory MendelsonReduction Gamma} {cpGamma: ClassicalPropositionalLogic L Gamma} (Phi: context) (x y: expr),
+Lemma contradiction_rule: forall {L: Language} {nL: NormalLanguage L} {pL: PropositionalLanguage L} {Gamma: ProofTheory L} {nGamma: NormalProofTheory L Gamma} {mpGamma: MinimunPropositionalLogic L Gamma} {cpGamma: ClassicalPropositionalLogic L Gamma} (Phi: context) (x y: expr),
   Phi |-- ~~ x ->
   Phi |-- x ->
   Phi |-- y.
@@ -37,7 +38,7 @@ Proof.
   auto.
 Qed.
 
-Lemma double_negp_add: forall {L: Language} {nL: NormalLanguage L} {pL: PropositionalLanguage L} {Gamma: ProofTheory L} {nGamma: NormalProofTheory L Gamma} {mpGamma: MinimunPropositionalLogic L Gamma} {rcGamma: ReductionConsistentProofTheory MendelsonReduction Gamma} {cpGamma: ClassicalPropositionalLogic L Gamma} (Phi: context) (x: expr),
+Lemma double_negp_add: forall {L: Language} {nL: NormalLanguage L} {pL: PropositionalLanguage L} {Gamma: ProofTheory L} {nGamma: NormalProofTheory L Gamma} {mpGamma: MinimunPropositionalLogic L Gamma} {cpGamma: ClassicalPropositionalLogic L Gamma} (Phi: context) (x: expr),
   Phi |-- ~~ (~~ x) --> x.
 Proof.
   intros.
@@ -48,7 +49,7 @@ Proof.
   auto.
 Qed.
 
-Lemma double_negp_elim: forall {L: Language} {nL: NormalLanguage L} {pL: PropositionalLanguage L} {Gamma: ProofTheory L} {nGamma: NormalProofTheory L Gamma} {mpGamma: MinimunPropositionalLogic L Gamma} {rcGamma: ReductionConsistentProofTheory MendelsonReduction Gamma} {cpGamma: ClassicalPropositionalLogic L Gamma} (Phi: context) (x: expr),
+Lemma double_negp_elim: forall {L: Language} {nL: NormalLanguage L} {pL: PropositionalLanguage L} {Gamma: ProofTheory L} {nGamma: NormalProofTheory L Gamma} {mpGamma: MinimunPropositionalLogic L Gamma} {cpGamma: ClassicalPropositionalLogic L Gamma} (Phi: context) (x: expr),
   Phi |-- x --> ~~ ~~ x.
 Proof.
   intros.
@@ -59,7 +60,7 @@ Proof.
   auto.
 Qed.
 
-Lemma contrapositivePP: forall {L: Language} {nL: NormalLanguage L} {pL: PropositionalLanguage L} {Gamma: ProofTheory L} {nGamma: NormalProofTheory L Gamma} {mpGamma: MinimunPropositionalLogic L Gamma} {rcGamma: ReductionConsistentProofTheory MendelsonReduction Gamma} {cpGamma: ClassicalPropositionalLogic L Gamma} Phi (x y: expr),
+Lemma contrapositivePP: forall {L: Language} {nL: NormalLanguage L} {pL: PropositionalLanguage L} {Gamma: ProofTheory L} {nGamma: NormalProofTheory L Gamma} {mpGamma: MinimunPropositionalLogic L Gamma} {cpGamma: ClassicalPropositionalLogic L Gamma} Phi (x y: expr),
   Phi |-- ~~ y --> ~~ x ->
   Phi |-- x --> y.
 Proof.
@@ -74,7 +75,7 @@ Proof.
   auto.
 Qed.
 
-Lemma contrapositiveNN: forall {L: Language} {nL: NormalLanguage L} {pL: PropositionalLanguage L} {Gamma: ProofTheory L} {nGamma: NormalProofTheory L Gamma} {mpGamma: MinimunPropositionalLogic L Gamma} {rcGamma: ReductionConsistentProofTheory MendelsonReduction Gamma} {cpGamma: ClassicalPropositionalLogic L Gamma} Phi (x y: expr),
+Lemma contrapositiveNN: forall {L: Language} {nL: NormalLanguage L} {pL: PropositionalLanguage L} {Gamma: ProofTheory L} {nGamma: NormalProofTheory L Gamma} {mpGamma: MinimunPropositionalLogic L Gamma} {cpGamma: ClassicalPropositionalLogic L Gamma} Phi (x y: expr),
   Phi |-- y --> x ->
   Phi |-- ~~ x --> ~~ y.
 Proof.
@@ -86,7 +87,7 @@ Proof.
   apply derivable_weaken1; eauto.
 Qed.
 
-Lemma contrapositiveNP: forall {L: Language} {nL: NormalLanguage L} {pL: PropositionalLanguage L} {Gamma: ProofTheory L} {nGamma: NormalProofTheory L Gamma} {mpGamma: MinimunPropositionalLogic L Gamma} {rcGamma: ReductionConsistentProofTheory MendelsonReduction Gamma} {cpGamma: ClassicalPropositionalLogic L Gamma} Phi (x y: expr),
+Lemma contrapositiveNP: forall {L: Language} {nL: NormalLanguage L} {pL: PropositionalLanguage L} {Gamma: ProofTheory L} {nGamma: NormalProofTheory L Gamma} {mpGamma: MinimunPropositionalLogic L Gamma} {cpGamma: ClassicalPropositionalLogic L Gamma} Phi (x y: expr),
   Phi |-- ~~ y --> x ->
   Phi |-- ~~ x --> y.
 Proof.
@@ -97,7 +98,7 @@ Proof.
   apply deduction_theorem; auto.
 Qed.
 
-Lemma contrapositivePN: forall {L: Language} {nL: NormalLanguage L} {pL: PropositionalLanguage L} {Gamma: ProofTheory L} {nGamma: NormalProofTheory L Gamma} {mpGamma: MinimunPropositionalLogic L Gamma} {rcGamma: ReductionConsistentProofTheory MendelsonReduction Gamma} {cpGamma: ClassicalPropositionalLogic L Gamma} Phi (x y: expr),
+Lemma contrapositivePN: forall {L: Language} {nL: NormalLanguage L} {pL: PropositionalLanguage L} {Gamma: ProofTheory L} {nGamma: NormalProofTheory L Gamma} {mpGamma: MinimunPropositionalLogic L Gamma} {cpGamma: ClassicalPropositionalLogic L Gamma} Phi (x y: expr),
   Phi |-- y --> ~~ x ->
   Phi |-- x --> ~~ y.
 Proof.
@@ -108,7 +109,7 @@ Proof.
   apply derivable_weaken1; auto.
 Qed.
 
-Lemma assum_exclude_middle: forall {L: Language} {nL: NormalLanguage L} {pL: PropositionalLanguage L} {Gamma: ProofTheory L} {nGamma: NormalProofTheory L Gamma} {mpGamma: MinimunPropositionalLogic L Gamma} {rcGamma: ReductionConsistentProofTheory MendelsonReduction Gamma} {cpGamma: ClassicalPropositionalLogic L Gamma} (Phi: context) (x y: expr),
+Lemma assum_exclude_middle: forall {L: Language} {nL: NormalLanguage L} {pL: PropositionalLanguage L} {Gamma: ProofTheory L} {nGamma: NormalProofTheory L Gamma} {mpGamma: MinimunPropositionalLogic L Gamma} {cpGamma: ClassicalPropositionalLogic L Gamma} (Phi: context) (x y: expr),
   Phi |-- ~~ x --> y ->
   Phi |-- x --> y ->
   Phi |-- y.
@@ -236,12 +237,9 @@ Inductive provable: expr -> Prop :=
 | true_provable: provable TT.
 (* Elliott Mendelson, Introduction to Mathematical Logic, Second Edition (New York: D. Van Nostrand, 1979) *)
 
-Instance AG: AxiomaticProofTheory.AxiomaticProofTheory L :=
-  AxiomaticProofTheory.Build_AxiomaticProofTheory L provable.
+Instance G: ProofTheory L := Build_AxiomaticProofTheory provable.
 
-Instance G: ProofTheory L := AxiomaticProofTheory.G AG.
-
-Instance nG: NormalProofTheory L G := AxiomaticProofTheory.nG AG.
+Instance nG: NormalProofTheory L G := Build_nAxiomaticProofTheory provable.
 
 Instance mpG: MinimunPropositionalLogic L G.
 Proof.
