PropositionalLogic/IntuitionisticPropositionalLogic.v
@@ -1,14 +1,15 @@
 Require Import Coq.Logic.Classical_Prop.
 Require Import Logic.lib.Coqlib.
 Require Import Logic.LogicBase.
-Require Import Logic.SyntacticReduction.
+Require Import Logic.MinimunLogic.MinimunLogic.
+Require Import Logic.MinimunLogic.SyntacticReduction.
+Require Import Logic.MinimunLogic.ContextProperty.
 Require Import Logic.PropositionalLogic.Syntax.
-Require Import Logic.PropositionalLogic.MinimunPropositionalLogic.
 
 Local Open Scope logic_base.
 Local Open Scope PropositionalLogic.
 
-Class IntuitionisticPropositionalLogic (L: Language) {nL: NormalLanguage L} {pL: PropositionalLanguage L} (Gamma: ProofTheory L) {mpGamma: MinimunPropositionalLogic L Gamma} {rcGamma: ReductionConsistentProofTheory IntuitionisticReduction Gamma} := {
+Class IntuitionisticPropositionalLogic (L: Language) {nL: NormalLanguage L} {pL: PropositionalLanguage L} (Gamma: ProofTheory L) {mpGamma: MinimunPropositionalLogic L Gamma} := {
   andp_intros: forall x y, |-- x --> y --> x && y;
   andp_elim1: forall x y, |-- x && y --> x;
   andp_elim2: forall x y, |-- x && y --> y;
@@ -18,7 +19,7 @@ Class IntuitionisticPropositionalLogic (L: Language) {nL: NormalLanguage L} {pL:
   falsep_elim: forall x, |-- FF --> x
 }.
 
-Lemma andp_intros_derivable: forall {L: Language} {nL: NormalLanguage L} {pL: PropositionalLanguage L} {Gamma: ProofTheory L} {nGamma: NormalProofTheory L Gamma} {mpGamma: MinimunPropositionalLogic L Gamma} {rcGamma: ReductionConsistentProofTheory IntuitionisticReduction Gamma} {ipGamma: IntuitionisticPropositionalLogic L Gamma} (Phi: context) (x y: expr),
+Lemma andp_intros_derivable: forall {L: Language} {nL: NormalLanguage L} {pL: PropositionalLanguage L} {Gamma: ProofTheory L} {nGamma: NormalProofTheory L Gamma} {mpGamma: MinimunPropositionalLogic L Gamma} {ipGamma: IntuitionisticPropositionalLogic L Gamma} (Phi: context) (x y: expr),
   Phi |-- x --> y --> x && y.
 Proof.
   intros.
@@ -28,7 +29,7 @@ Proof.
   intros ? [].
 Qed.
 
-Lemma andp_elim1_derivable: forall {L: Language} {nL: NormalLanguage L} {pL: PropositionalLanguage L} {Gamma: ProofTheory L} {nGamma: NormalProofTheory L Gamma} {mpGamma: MinimunPropositionalLogic L Gamma} {rcGamma: ReductionConsistentProofTheory IntuitionisticReduction Gamma} {ipGamma: IntuitionisticPropositionalLogic L Gamma} (Phi: context) (x y: expr),
+Lemma andp_elim1_derivable: forall {L: Language} {nL: NormalLanguage L} {pL: PropositionalLanguage L} {Gamma: ProofTheory L} {nGamma: NormalProofTheory L Gamma} {mpGamma: MinimunPropositionalLogic L Gamma} {ipGamma: IntuitionisticPropositionalLogic L Gamma} (Phi: context) (x y: expr),
   Phi |-- x && y --> x.
 Proof.
   intros.
@@ -38,7 +39,7 @@ Proof.
   intros ? [].
 Qed.
 
-Lemma andp_elim2_derivable: forall {L: Language} {nL: NormalLanguage L} {pL: PropositionalLanguage L} {Gamma: ProofTheory L} {nGamma: NormalProofTheory L Gamma} {mpGamma: MinimunPropositionalLogic L Gamma} {rcGamma: ReductionConsistentProofTheory IntuitionisticReduction Gamma} {ipGamma: IntuitionisticPropositionalLogic L Gamma} (Phi: context) (x y: expr),
+Lemma andp_elim2_derivable: forall {L: Language} {nL: NormalLanguage L} {pL: PropositionalLanguage L} {Gamma: ProofTheory L} {nGamma: NormalProofTheory L Gamma} {mpGamma: MinimunPropositionalLogic L Gamma} {ipGamma: IntuitionisticPropositionalLogic L Gamma} (Phi: context) (x y: expr),
   Phi |-- x && y --> y.
 Proof.
   intros.
@@ -48,7 +49,7 @@ Proof.
   intros ? [].
 Qed.
 
-Lemma orp_intros1_derivable: forall {L: Language} {nL: NormalLanguage L} {pL: PropositionalLanguage L} {Gamma: ProofTheory L} {nGamma: NormalProofTheory L Gamma} {mpGamma: MinimunPropositionalLogic L Gamma} {rcGamma: ReductionConsistentProofTheory IntuitionisticReduction Gamma} {ipGamma: IntuitionisticPropositionalLogic L Gamma} (Phi: context) (x y: expr),
+Lemma orp_intros1_derivable: forall {L: Language} {nL: NormalLanguage L} {pL: PropositionalLanguage L} {Gamma: ProofTheory L} {nGamma: NormalProofTheory L Gamma} {mpGamma: MinimunPropositionalLogic L Gamma} {ipGamma: IntuitionisticPropositionalLogic L Gamma} (Phi: context) (x y: expr),
   Phi |-- x --> x || y.
 Proof.
   intros.
@@ -58,7 +59,7 @@ Proof.
   intros ? [].
 Qed.
 
-Lemma orp_intros2_derivable: forall {L: Language} {nL: NormalLanguage L} {pL: PropositionalLanguage L} {Gamma: ProofTheory L} {nGamma: NormalProofTheory L Gamma} {mpGamma: MinimunPropositionalLogic L Gamma} {rcGamma: ReductionConsistentProofTheory IntuitionisticReduction Gamma} {ipGamma: IntuitionisticPropositionalLogic L Gamma} (Phi: context) (x y: expr),
+Lemma orp_intros2_derivable: forall {L: Language} {nL: NormalLanguage L} {pL: PropositionalLanguage L} {Gamma: ProofTheory L} {nGamma: NormalProofTheory L Gamma} {mpGamma: MinimunPropositionalLogic L Gamma} {ipGamma: IntuitionisticPropositionalLogic L Gamma} (Phi: context) (x y: expr),
   Phi |-- y --> x || y.
 Proof.
   intros.
@@ -68,7 +69,7 @@ Proof.
   intros ? [].
 Qed.
 
-Lemma orp_elim_derivable: forall {L: Language} {nL: NormalLanguage L} {pL: PropositionalLanguage L} {Gamma: ProofTheory L} {nGamma: NormalProofTheory L Gamma} {mpGamma: MinimunPropositionalLogic L Gamma} {rcGamma: ReductionConsistentProofTheory IntuitionisticReduction Gamma} {ipGamma: IntuitionisticPropositionalLogic L Gamma} (Phi: context) (x y z: expr),
+Lemma orp_elim_derivable: forall {L: Language} {nL: NormalLanguage L} {pL: PropositionalLanguage L} {Gamma: ProofTheory L} {nGamma: NormalProofTheory L Gamma} {mpGamma: MinimunPropositionalLogic L Gamma} {ipGamma: IntuitionisticPropositionalLogic L Gamma} (Phi: context) (x y z: expr),
   Phi |-- (x --> z) --> (y --> z) --> (x || y --> z).
 Proof.
   intros.
@@ -78,7 +79,7 @@ Proof.
   intros ? [].
 Qed.
 
-Lemma falsep_elim_derivable: forall {L: Language} {nL: NormalLanguage L} {pL: PropositionalLanguage L} {Gamma: ProofTheory L} {nGamma: NormalProofTheory L Gamma} {mpGamma: MinimunPropositionalLogic L Gamma} {rcGamma: ReductionConsistentProofTheory IntuitionisticReduction Gamma} {ipGamma: IntuitionisticPropositionalLogic L Gamma} (Phi: context) (x: expr),
+Lemma falsep_elim_derivable: forall {L: Language} {nL: NormalLanguage L} {pL: PropositionalLanguage L} {Gamma: ProofTheory L} {nGamma: NormalProofTheory L Gamma} {mpGamma: MinimunPropositionalLogic L Gamma} {ipGamma: IntuitionisticPropositionalLogic L Gamma} (Phi: context) (x: expr),
   Phi |-- FF --> x.
 Proof.
   intros.
@@ -88,7 +89,7 @@ Proof.
   intros ? [].
 Qed.
 
-Lemma DCS_andp_iff: forall {L: Language} {nL: NormalLanguage L} {pL: PropositionalLanguage L} {Gamma: ProofTheory L} {nGamma: NormalProofTheory L Gamma} {mpGamma: MinimunPropositionalLogic L Gamma} {rcGamma: ReductionConsistentProofTheory IntuitionisticReduction Gamma} {ipGamma: IntuitionisticPropositionalLogic L Gamma} (Phi: context),
+Lemma DCS_andp_iff: forall {L: Language} {nL: NormalLanguage L} {pL: PropositionalLanguage L} {Gamma: ProofTheory L} {nGamma: NormalProofTheory L Gamma} {mpGamma: MinimunPropositionalLogic L Gamma} {ipGamma: IntuitionisticPropositionalLogic L Gamma} (Phi: context),
   derivable_closed Phi ->
   (forall x y: expr, Phi (x && y) <-> (Phi x /\ Phi y)).
 Proof.
@@ -104,7 +105,7 @@ Proof.
     apply derivable_modus_ponens with x; auto.
 Qed.
 
-Lemma DCS_orp_iff: forall {L: Language} {nL: NormalLanguage L} {pL: PropositionalLanguage L} {Gamma: ProofTheory L} {nGamma: NormalProofTheory L Gamma} {mpGamma: MinimunPropositionalLogic L Gamma} {rcGamma: ReductionConsistentProofTheory IntuitionisticReduction Gamma} {ipGamma: IntuitionisticPropositionalLogic L Gamma} (Phi: context),
+Lemma DCS_orp_iff: forall {L: Language} {nL: NormalLanguage L} {pL: PropositionalLanguage L} {Gamma: ProofTheory L} {nGamma: NormalProofTheory L Gamma} {mpGamma: MinimunPropositionalLogic L Gamma} {ipGamma: IntuitionisticPropositionalLogic L Gamma} (Phi: context),
   derivable_closed Phi ->
   orp_witnessed Phi ->
   (forall x y: expr, Phi (x || y) <-> (Phi x \/ Phi y)).
@@ -145,10 +146,9 @@ Inductive provable: expr -> Prop :=
 | orp_elim: forall x y z, provable ((x --> z) --> (y --> z) --> (x || y --> z))
 | falsep_elim: forall x, provable (FF --> x).
 
-Instance AG: AxiomaticProofTheory.AxiomaticProofTheory L :=
-  AxiomaticProofTheory.Build_AxiomaticProofTheory L provable.
+Instance G: ProofTheory L := Build_AxiomaticProofTheory provable.
 
-Instance G: ProofTheory L := AxiomaticProofTheory.G AG.
+Instance nG: NormalProofTheory L G := Build_nAxiomaticProofTheory provable.
 
 Instance mpG: MinimunPropositionalLogic L G.
 Proof.
