MinimunLogic/ContextProperty.v
@@ -1,0 +1,73 @@
+Require Import Logic.LogicBase.
+Require Import Logic.lib.Coqlib.
+Require Import Logic.MinimunLogic.MinimunLogic.
+
+Local Open Scope logic_base.
+
+Definition consistent {L: Language} {nL: NormalLanguage L} {Gamma: ProofTheory L}: context -> Prop :=
+  fun Phi => ~ derivable Phi falsep.
+
+Definition maximal_consistent {L: Language} {nL: NormalLanguage L} {Gamma: ProofTheory L}: context -> Prop :=
+  fun Phi => consistent Phi /\ forall Psi, consistent Psi -> Included _ Phi Psi -> Included _ Psi Phi.
+
+Definition derivable_closed {L: Language} {nL: NormalLanguage L} {Gamma: ProofTheory L}: context -> Prop :=
+  fun Phi => forall x, derivable Phi x -> Phi x.
+
+Lemma maximal_consistent_spec {L: Language} {nL: NormalLanguage L} {Gamma: ProofTheory L} {nGamma: NormalProofTheory L Gamma}:
+  forall Phi, maximal_consistent Phi <-> consistent Phi /\ forall x, consistent (Union _ Phi (Singleton _ x)) -> Phi x.
+Proof.
+  intros.
+  split; intros [? ?]; split; auto.
+  + intros.
+    specialize (H0 _ H1).
+    specialize (H0 (fun x H => Union_introl _ _ _ _ H)).
+    specialize (H0 x).
+    apply H0; right; constructor.
+  + intros.
+    hnf; intros.
+    apply H0.
+    unfold consistent in*.
+    intro; apply H1.
+    eapply derivable_weaken; [| exact H4].
+    intros ? [? | ?]; auto.
+    intros []; auto.
+Qed.
+
+Lemma derivable_closed_element_derivable: forall {L: Language} {nL: NormalLanguage L} {Gamma: ProofTheory L} {nGamma: NormalProofTheory L Gamma} {mpGamma: MinimunPropositionalLogic L Gamma} (Phi: context),
+  derivable_closed Phi ->
+  (forall x: expr, Phi x <-> Phi |-- x).
+Proof.
+  intros.
+  split; intros; auto.
+  apply derivable_assum; auto.
+Qed.
+
+Lemma maximal_consistent_derivable_closed: forall {L: Language} {nL: NormalLanguage L} {Gamma: ProofTheory L} {nGamma: NormalProofTheory L Gamma} {mpGamma: MinimunPropositionalLogic L Gamma} (Phi: context),
+  maximal_consistent Phi ->
+  derivable_closed Phi.
+Proof.
+  intros.
+  hnf; intros.
+  assert (consistent (Union _ Phi (Singleton _ x))).
+  Focus 1. {
+    intro.
+    pose proof impp_elim _ _ _ H1.
+    pose proof derivable_modus_ponens _ _ _ H0 H2.
+    destruct H; auto.
+  } Unfocus.
+  destruct H.
+  specialize (H2 _ H1).
+  specialize (H2 (fun x H => Union_introl _ _ _ x H)).
+  apply H2.
+  right; constructor.
+Qed.
+
+Lemma MCS_element_derivable: forall {L: Language} {nL: NormalLanguage L} {Gamma: ProofTheory L} {nGamma: NormalProofTheory L Gamma} {mpGamma: MinimunPropositionalLogic L Gamma} (Phi: context),
+  maximal_consistent Phi ->
+  (forall x: expr, Phi x <-> Phi |-- x).
+Proof.
+  intros.
+  apply derivable_closed_element_derivable, maximal_consistent_derivable_closed.
+  auto.
+Qed.
+
