PropositionalLogic/Sound_Classical_Trivial.v
@@ -1,5 +1,7 @@
 Require Import Logic.LogicBase.
-Require Import Logic.SyntacticReduction.
+Require Import Logic.MinimunLogic.MinimunLogic.
+Require Import Logic.MinimunLogic.SyntacticReduction.
+Require Import Logic.MinimunLogic.ContextProperty.
 Require Import Logic.PropositionalLogic.Syntax.
 Require Import Logic.PropositionalLogic.ClassicalPropositionalLogic.
 Require Import Logic.PropositionalLogic.TrivialSemantics.
